%%%%%%%%%%%%%%%%%%%%%%%%%%%%%%%%%%%%%%%%%
% Author: Sibi <sibi@psibi.in>
%%%%%%%%%%%%%%%%%%%%%%%%%%%%%%%%%%%%%%%%%
\documentclass{article}
\usepackage{graphicx}
\usepackage{verbatim}
\usepackage{amsmath}
\usepackage{amsfonts}
\usepackage{amssymb}
\usepackage{tabularx}
\setlength\parskip{\baselineskip}
\begin{document}
\title{Chapter 3 (Section 3.2)}
\author{Sibi}
\date{\today}
\maketitle
\newpage

\section{Problem 1}

Solution (a)

%% +--------------+--------------+
%% |Givens        |Goals         |
%% +--------------+--------------+
%% |P \implies Q  |P \implies R  |
%% |              |              |
%% |Q \implies R  |              |
%% +--------------+--------------+
% This LaTeX table template is generated by emacs 24.3.1
\begin{tabular}{| >{$}l<{$} | >{$}l<{$} |}
\hline
Givens & Goals \\
\hline
P \implies Q & P \implies R \\
 & \\
Q \implies R & \\
\hline
\end{tabular}


%% +--------------+--------------+
%% |Givens        |Goals         |
%% +--------------+--------------+
%% |P \implies Q  |R             |
%% |              |              |
%% |Q \implies R  |              |
%% |              |              |
%% |P             |              |
%% +--------------+--------------+
% This LaTeX table template is generated by emacs 24.3.1
\begin{tabular}{| >{$}l<{$} | >{$}l<{$} |}
\hline
Givens & Goals \\
\hline
P \implies Q & R \\
 & \\
Q \implies R & \\
 & \\
P & \\
\hline
\end{tabular}

Proof Structure

Suppose $P$.

   [Proof of R goes here]
   
Therefore $P \implies R$.

Proof. Suppose $P$. Since $P \implies Q$, using modus ponens we can
conclude $Q$. Since $Q \implies R$, again from modus ponens we can
conclude R. Therefore, $P \implies R$.

Solution (b)

%% +--------------------+--------------+
%% |Givens              |Goals         |
%% +--------------------+--------------+
%% |\neg R \implies (P  |P \implies (Q |
%% |\implies \neg Q)    |\implies R)   |
%% +--------------------+--------------+
% This LaTeX table template is generated by emacs 24.3.1
\begin{tabular}{| >{$}l<{$} | >{$}l<{$} |}
\hline
Givens & Goals \\
\hline
\neg R \implies (P & P \implies (Q \\
\implies \neg Q) & \implies R) \\
\hline
\end{tabular}

$ \neg R \implies (P \implies \neg Q)$ is equivalent to $(P \land Q)
\implies R$

Proof. Suppose P. Suppose Q. Since $ \neg R \implies (P \implies \neg
Q) $ is equivalent to $(P \land Q) \implies R$, we can conclude R.
Therefore, $P \implies (Q \implies R)$.

\section{Problem 2}

Solution(a)

Proof. Suppose P. Since $P \implies Q$, we can conclude Q. Since $R
\implies \neg Q$ is equivalent to $Q \implies \neg R$, we can conclude
$\neg R$ as Q is true. Therefore, $P \implies \neg R$ is true.

Solution (b)

Proof. Suppose Q. We will prove by contradiction. Let $Q \implies \neg
P$ be true. But $\neg P$ is true but our given $P$ is also true which
leads us to a contradiction. Therefore, $\neg(Q \implies \neg P)$ is
true.

Alt. Proof: Suppose $Q$. Then $\neg (Q \implies \neg P) \equiv Q \land P$,
because $\neg (Q \implies \neg P) \equiv \neg ( \neg Q \lor \neg P )$.
Since we are given P and assumed Q, then $Q \land  P$ is true, 
therefore if $P$ and $Q$ are true then $Q \implies \neg (Q \implies \neg P)$ 
is also true.

\section{Problem 3}

Proof. Suppse $x \in A$. Since $A \subseteq C$, it follows $x \in C$.
But B and C are disjoint, so $x \notin B$.

Expanded Proof. Suppose $x \in A$. Since $A \subseteq C$ then it holds that
$x \in A \implies x \in C$, so $x \in C$. Since $B \cap C = \emptyset$ then
$x \in C \implies x \notin B$, therefore $x \notin B$.

\section{Problem 4}

Proof. Suppose $x \in C$. We can conclude that $x \notin A \setminus
B$. From, $x \notin A \setminus B$, it follows that $x \in B$.
Therefore, if $x \in C$, then $x \in B$.

\section{Problem 5}

Proof. (by contradiction) Suppose $a \in A \setminus B$. 
It follows that $a \in A$ from our assumption. Also,
$a \in C$ from which we can conclude that $a \in B$ since $A \cap C
\subseteq B$ But this contradicts the fact that $a \notin B$.
Therefore $a \notin A \setminus B$.

\section{Problem 6}

Proof. (by contradiction) Suppose $a \notin C$. From $a
\notin B \setminus C$, we can conclude that either $a \notin B$ or $a
\in C$ is true. Since $a \in A$, we can conclude that $a \in B$ from
$A \subseteq B$. So, $a \notin B$ is false. Therefore, $a \in C$
should be true. But this contradicts the fact that $a \notin C$.
Therefore $a \in C$.

Note: This can be proven by focusing on $a \in B$ as well. By assuming
$a \notin C$ we know that $a \notin B$ by $a \notin B \setminus C$, since this
means logically that $\neg (a \in B \land a \notin C)$ which simplifies
to $a \notin B \lor a \in C$. By assuming $a \notin C$ we automatically
must have $a \notin B$. But since we have $a \in A$ then by the subset
$A \subseteq B$ we have $\forall x ( x \in A \implies x \in B)$ and
therefore $a \in A$ is sufficient to force $a \in B$. But this
contradicts that $a$ cannot be in $B$ since we assumed $a \notin C$.
Since $a \notin C$ causes an impossible situation, $a$ must be in $C$.

\section{Problem 7}

Proof. (by contradiction) Suppose $y = 0$. Solving $y +
x = 2y - x$ by substituting $y=0$ we get that $x=0$. But it
contradicts the fact that both $x$ and $y$ cannot be $0$. Therefore,
$y \neq 0$.

\section{Problem 8}

Proof. Suppose $a < 1/a < b < 1/b$. Multiplying  the inequality by
$1/a < 1/b$ by $ab$ we should get $a < b$. From this, we can conclude
that $ab$ is a negative number. Since $a < b$, we can conclude that
$a$ is the negative number. Multiplying inequality $a < 1/a$ by
negative number we get $a^2 < 1$. From that we can conclude that $a <
-1$. Therefore, if $a < 1/a < b < 1/b$, then $a < -1$.

\section{Problem 9}

Proof. (by contradiction) Suppose $x^2y = 2x + y$. Suppose $y \neq 0$ Suppose $x = 0$.
Substituting this into the equivalent $x^2y = 2x + y$, we get $y = 0$.
But this contradicts the fact that $y \neq 0$. Therefore $x \neq 0$.
Thus, if $y \neq 0$, then $x \neq 0$.

\section{Problem 10}

Proof. Suppose $x \neq 0$. Suppose $y = 3x^2 + 2y / x^2 + 2$. Solving
it we get $x^2(3 - y) = 0$. Since $x \neq 0$, we can conclude that $y
= 3$.

\section{Problem 11}

Solution (a)

If conclusion of the theorem is false, then $\neg( x \neq 3 \land y
\neq 8)$. That is equivalent to $x = 3 \lor y = 8$.

Solution (b)

First example: $x = 3$ and $y = 7$.
Second example: $x = 2$ and $y = 8$.

\section{Problem 12}

Solution (a)

This is plain wrong: Since $x \notin B$ and $B \subseteq C$, $x \notin
C$.

From $x \notin B$ and $B \subseteq C$, we cannot conclude that $x
\notin C$.

Expansion:

$A \subseteq C$ means $\forall x ( x \in A \implies x \in B )$. Likewise,
$B \subseteq C$ means $\forall x ( x \in B \implies x \in C )$. We are given
that $x \in A$, therefore we know $x \in C$ by the first given. Now if we
claim that $x \notin C$ because $x \notin B$ then we are committing the 
fallacy of denying the hypothesis, or trying to accept the inverse of
$x \in B \implies x \in C$. This is clearly wrong, therefore the proof
is invalid.

Solution (b)

$ C = \{1,2,3,4,5\} $
$ A = \{1,2\}$
$ B = \{3,4,5\}$
$ x = 1 $

\subsection{Problem 13}
Hypotheses:
\begin{itemize}
\item $P \rightarrow Q$
\item $\lnot Q$
\end{itemize}
Conclusion: then $\lnot P$.\\
\begin{table}[h!]
\begin{tabular}{c|c|c|c|c}
$P$ & $Q$ & $\lnot Q$ & $P \rightarrow Q$ & $\lnot P$ \\\hline
1 & 1 & 0 & 1 & 0\\
1 & 0 & 1 & 0 & 0\\
0 & 1 & 0 & 1 & 1\\\hline
\textbf{0} & \textbf{0} & \textbf{1} & \textbf{1} & \textbf{1}\\\hline
\end{tabular}
\end{table}
\newpage
\subsection{Problem 14}
Truth table for 3.2.4
\begin{table}[h!]
\begin{tabular}{c|c|c|c|c}
$P$ & $Q$ & $R$ & $P \rightarrow (Q \rightarrow R)$ & $\lnot R \rightarrow (P \rightarrow \lnot Q)$ \\\hline
0 & 0 & 0 & 1 & 1\\
0 & 0 & 1 & 1 & 1\\
0 & 1 & 0 & 1 & 1\\
0 & 1 & 1 & 1 & 1\\
1 & 0 & 0 & 1 & 1\\
1 & 0 & 1 & 1 & 1\\
1 & 1 & 0 & 0 & 0\\
1 & 1 & 1 & 1 & 1
\end{tabular}
\end{table}

\subsection{Problem 15}
(a)
\begin{table}[h!]
\begin{tabular}{c|c|c|c|c|c}
$P$ & $Q$ & $R$ & $P \rightarrow Q$ & $Q \rightarrow R$ & $P\rightarrow R$\\\hline
0 & 0 & 0 & 1 & 1 & 1\\
0 & 0 & 1 & 1 & 1 & 1\\
0 & 1 & 0 & 1 & 0 & 1\\
0 & 1 & 1 & 1 & 1 & 1\\
1 & 0 & 0 & 0 & 1 & 0\\
1 & 0 & 1 & 0 & 1 & 1\\
1 & 1 & 0 & 1 & 0 & 0\\
1 & 1 & 1 & 1 & 1 & 1
\end{tabular}
\end{table}\\
(b)
\begin{table}[h!]
\begin{tabular}{c|c|c|c|c}
$P$ & $Q$ & $R$ & $\lnot R \rightarrow (P \rightarrow \lnot Q)$ & $P \rightarrow (Q \rightarrow R)$ \\\hline
0 & 0 & 0 & 1 & 1\\
0 & 0 & 1 & 1 & 1\\
0 & 1 & 0 & 1 & 1\\
0 & 1 & 1 & 1 & 1\\
1 & 0 & 0 & 1 & 1\\
1 & 0 & 1 & 1 & 1\\
1 & 1 & 0 & 0 & 0\\
1 & 1 & 1 & 1 & 1
\end{tabular}
\end{table}
\newpage
\subsection{Problem 16}
(a)\\
\begin{tabular}{c|c|c|c|c|c}
$P$ & $Q$ & $R$ & $P \rightarrow Q$ & $R \rightarrow \lnot Q$ & $P \rightarrow \lnot R$\\\hline
0 & 0 & 0 & 1 & 1 & 1\\
0 & 0 & 1 & 1 & 1 & 1\\
0 & 1 & 0 & 1 & 1 & 1\\
0 & 1 & 1 & 1 & 0 & 1\\
1 & 0 & 0 & 0 & 1 & 1\\
1 & 0 & 1 & 0 & 1 & 0\\
1 & 1 & 0 & 1 & 1 & 1\\
1 & 1 & 1 & 1 & 0 & 0
\end{tabular}\\
(b)
\begin{table}[h!]
\begin{tabular}{c|c|c|c}
$P$ & $Q$ & $P$ & $Q \rightarrow \lnot (Q \rightarrow \lnot P)$ \\\hline
0 & 0 & 0 & 1\\
0 & 1 & 0 & 0\\
1 & 0 & 1 & 1\\
1 & 1 & 1 & 1 
\end{tabular}
\end{table}\

\subsection{Problem 17}
No. If we assume $y=4$ and substitute into the equation ($x^2+4=13 \equiv x = \pm 3$) we get $x=-3$. Such that $y=4$ and $x=-3$ is a counterexample to the theorem.
\end{document}
